new/experiments/store.v
@@ -1,0 +1,129 @@
+From New.proof Require Import grove_prelude.
+
+Section proof.
+Context `{!heapGS Σ}.
+
+Definition test (l : loc) : expr :=
+  do: #l <-[uint64T] #0 ;;;
+  do: #l <-[uint64T] #1 ;;;
+  do: #l <-[uint64T] #2 ;;;
+  do: #l <-[uint64T] #3 ;;;
+  do: #l <-[uint64T] #4 ;;;
+  do: #l <-[uint64T] #5 ;;;
+  do: #l <-[uint64T] #6 ;;;
+  do: #l <-[uint64T] #7 ;;;
+  do: #l <-[uint64T] #8 ;;;
+  do: #l <-[uint64T] #9
+.
+
+Axiom own_something : iProp Σ.
+
+Definition big_context l : iProp Σ :=
+  "Hown" ∷ l ↦[uint64T] #0 ∗
+  "H0" ∷ own_something ∗
+  "H1" ∷ own_something ∗
+  "H2" ∷ own_something ∗
+  "H3" ∷ own_something ∗
+  "H4" ∷ own_something ∗
+  "H5" ∷ own_something ∗
+  "H6" ∷ own_something ∗
+  "H7" ∷ own_something ∗
+  "H8" ∷ own_something ∗
+  "H9" ∷ own_something
+.
+
+Lemma x (l : loc) :
+  {{{ big_context l }}}
+    (test l)
+  {{{ RET (execute_val #()); True }}}.
+Proof.
+  iIntros (?) "H HΦ".
+  unfold test.
+  iNamed "H".
+  time (do 10 wp_store).
+  wp_pures.
+  by iApply "HΦ".
+Time Qed.
+(* Finished transaction in 2.695 secs (2.356u,0.s) (successful) *)
+
+
+Lemma tac_wp_store_ty_bad K Δ Δ''
+                          Δ1 Δ2 Δ3 Δ4 Δ5 Δ6 Δ7 Δ8 Δ9 Δ10
+                          Δ11 Δ12 Δ13 Δ14 Δ15 Δ16 Δ17 Δ18 Δ19 Δ20
+                          Δ21 Δ22 Δ23 Δ24 Δ25 Δ26 Δ27
+  stk E i l t v v' Φ :
+  (Δ = Δ1 ∧
+   Δ = Δ2 ∧
+   Δ = Δ3 ∧
+   Δ = Δ4 ∧
+   Δ = Δ5 ∧
+   Δ = Δ6 ∧
+   Δ = Δ7 ∧
+   Δ = Δ8 ∧
+   Δ = Δ9 ∧
+   Δ = Δ10 ∧
+   Δ = Δ11 ∧
+   Δ = Δ12 ∧
+   Δ = Δ13 ∧
+   Δ = Δ14 ∧
+   Δ = Δ15 ∧
+   Δ = Δ16 ∧
+   Δ = Δ17 ∧
+   Δ = Δ18 ∧
+   Δ = Δ19 ∧
+   Δ = Δ20 ∧
+   Δ = Δ21 ∧
+   Δ = Δ22 ∧
+   Δ = Δ23 ∧
+   Δ = Δ24 ∧
+   Δ = Δ25 ∧
+   Δ = Δ26 ∧
+   Δ = Δ27
+  ) →
+  has_go_type v' t ->
+  envs_lookup i Δ = Some (false, l ↦[t] v)%I →
+  envs_simple_replace i false (Esnoc Enil i (l ↦[t] v')) Δ = Some Δ'' →
+  envs_entails Δ'' (WP fill K (Val $ LitV LitUnit) @ stk; E {{ Φ }}) →
+  envs_entails Δ (WP fill K (store_ty t (PairV (LitV l) v')) @ stk; E {{ Φ }}).
+Proof.
+Admitted.
+
+Tactic Notation "wp_store_bad" :=
+  let solve_pointsto _ :=
+    let l := match goal with |- _ = Some (_, (?l ↦[_] _)%I) => l end in
+    iAssumptionCore || fail "wp_store: cannot find" l "↦[t] ?" in
+  wp_pures;
+  lazymatch goal with
+  | |- envs_entails _ (wp ?s ?E ?e ?Q) =>
+    first
+      [reshape_expr e ltac:(fun K e' => eapply (tac_wp_store_ty_bad K))
+      |fail 1 "wp_store: cannot find 'store_ty' in" e];
+    [done
+    |(repeat econstructor || fail "could not establish [has_go_type]") (* solve [has_go_type v' t] *)
+    |solve_pointsto ()
+    |reduction.pm_reflexivity
+    |first [wp_pure_filter (Rec BAnon BAnon _)|wp_finish]]
+  | _ => fail "wp_store: not a 'wp'"
+  end.
+
+Lemma x_bad (l : loc) :
+  {{{ big_context l }}}
+    (test l)
+  {{{ RET (execute_val #()); True }}}.
+Proof.
+  iIntros (?) "H HΦ".
+  unfold test.
+  iNamed "H".
+  wp_pures.
+  time (do 10 wp_store_bad).
+  wp_pures.
+  by iApply "HΦ".
+  Optimize Proof.
+  Optimize Heap.
+Time Qed.
+
+(* with 9 Δs: Finished transaction in 1.342 secs (1.336u,0.s) (successful) *)
+(* with 27 Δs: Finished transaction in 5.794 secs (5.785u,0.003s) (successful) *)
+Print x_bad.
+
+End proof.
