new/experiments/type.v
@@ -1,0 +1,153 @@
+From New.proof Require Import grove_prelude.
+
+Section definitions.
+
+Context `{!heapGS Σ}.
+
+Context {typ : Type}.
+Context {typ_eqb : typ → typ → bool}.
+
+Inductive prop :=
+| prop_own : nat → prop
+| prop_sep : prop → prop → prop
+| prop_wand : prop → prop → prop
+| prop_var : string → prop
+| prop_forall (x : string) (A : typ) : prop → prop
+.
+
+Fixpoint prop_eqb (P : prop) (Q : prop) : bool :=
+  match P, Q with
+  | prop_own n, prop_own m => Nat.eqb n m
+  | prop_sep P Q, prop_sep P' Q' => prop_eqb P P' && prop_eqb Q Q'
+  | prop_wand P Q, prop_wand P' Q' => prop_eqb P P' && prop_eqb Q Q'
+  | prop_var x, prop_var y => String.eqb x y
+
+  (* XXX: no α-conversion *)
+  | prop_forall x A P, prop_forall x' A' P'  => String.eqb x x' && typ_eqb A A' && prop_eqb P P'
+  | _, _ => false
+  end.
+
+Declare Scope prop_scope.
+Delimit Scope prop_scope with prop_scope.
+Notation "P ∗ Q" := (prop_sep P%prop_scope Q%prop_scope) : prop_scope.
+Notation "P -∗ Q" := (prop_wand P%prop_scope Q%prop_scope) : prop_scope.
+
+Bind Scope prop_scope with prop.
+
+Inductive term :=
+| cons_sep (el : term) (er : term) : term
+| lam (x : string) (e : term) : term
+| var (x : string)
+.
+
+Definition typing_context : Type := list (string * prop).
+
+Definition context_lookup := (assocl_lookup (A:=prop)).
+
+Fixpoint context_delete (s : string) (Γ : typing_context) : typing_context :=
+  match Γ with
+  | [] => []
+  | (n,P) :: Γ => if (String.eqb n s) then (context_delete s Γ) else (n,P) :: (context_delete s Γ)
+  end
+.
+
+Fixpoint has_type_internal (Γ : typing_context) (t : term) (P : prop) : (bool * typing_context) :=
+  match P, t with
+  | prop_sep P Q, cons_sep el er =>
+      let '(bl, Γ) := has_type_internal Γ el P in
+      let '(br, Γ) := has_type_internal Γ er Q in
+      (bl && br, Γ)
+  | prop_wand P Q, lam x e =>
+      has_type_internal ((x,P)::Γ) e Q
+  | _, var x => match (context_lookup x Γ) with
+               | Some P' => (prop_eqb P' P, context_delete x Γ)
+               | _ => (false, [])
+               end
+  | _, _ => (false, [])
+  end.
+
+Definition type_check (t : term) (P : prop) : bool := fst (has_type_internal [] t P).
+
+Definition proof : term :=
+  lam "HP" (lam "HQ" $ cons_sep (var "HP") (var "HQ")).
+
+Definition P := prop_own 10.
+Definition Q := prop_own 11.
+
+Eval compute in type_check proof (P -∗ Q -∗ (P ∗ Q)).
+
+Goal ∀ (P' Q': iProp Σ), P' -∗ Q' -∗ P' ∗ Q'.
+Proof.
+  iIntros (??) "$ $".
+  Show Proof.
+  Print proof.
+Qed.
+
+Lemma r S : prop_eqb S S = true.
+Proof.
+  induction S.
+  - simpl. by rewrite Nat.eqb_refl.
+  - simpl. rewrite IHS1 IHS2. done.
+  - simpl. rewrite IHS1 IHS2. done.
+  - simpl.
+Abort.
+
+Lemma general S T :
+  type_check proof (S -∗ T -∗ (S ∗ T)).
+Proof.
+  unfold type_check.
+  simpl.
+  Show Proof.
+Abort.
+
+Lemma tac_wand_intro (i : ident) (Δ : envs (iProp Σ)) (P Q : iProp Σ) :
+  match envs_app false (Esnoc Enil i P) Δ with
+  | Some Δ' => envs_entails Δ' Q
+  | None => False
+  end → envs_entails Δ (P -∗ Q)
+.
+Proof.
+Admitted.
+
+Fixpoint nwand n P : iProp Σ :=
+  match n with
+  | O => True
+  | S n => P -∗ (nwand n P)
+  end
+.
+
+Fixpoint nimpl n P : Prop :=
+  match n with
+  | O => True
+  | S n => P -> (nimpl n P)
+  end
+.
+
+Lemma test_impl P :
+  nimpl 1000 P
+.
+Proof.
+  repeat intros ?.
+  refine I.
+Time Qed.
+(* Finished transaction in 1.161 secs (1.16u,0.s) (successful) *)
+
+Lemma test P :
+  ⊢ nwand 100 P
+.
+Proof.
+  iStartProof.
+  repeat iIntros "?".
+  done.
+Time Qed.
+(*
+50: 0.042
+100: 0.167
+200: 0.682
+300: 1.765
+400: 3.192
+500: 4.973
+1000: 20.68
+ *)
+
+End definitions.
