new/experiments/unsound.v
@@ -1,0 +1,81 @@
+From New.code Require Import github_com.mit_pdos.gokv.lockservice.
+From New.proof Require Import grove_prelude.
+
+(* Takes a WP goal as input, and gives the next proof goal as output *)
+From Ltac2 Require Import Ltac2.
+Set Default Proof Mode "Classic".
+Import Ltac2.Message.
+
+Ltac2 mutable dbg := print.
+Ltac2 mutable dbg_constr c := print (of_constr c).
+
+Ltac2 simpl_flags := {
+    Std.rStrength := Std.Norm;
+  Std.rBeta := true;
+  Std.rMatch := true;
+  Std.rFix := true;
+  Std.rCofix := true;
+  Std.rZeta := true;
+  Std.rDelta := true ;
+  Std.rConst := []
+}.
+
+Ltac2 rec expr_step e : constr :=
+  lazy_match! e with
+  | Rec ?f ?x ?e =>
+      dbg (of_string "reached Rec");
+      '(Val $ RecV $f $x $e)
+  | App (Val (RecV ?f ?x ?e)) (Val ?v2) =>
+      dbg (of_string "reached App (RecV ...) v");
+      dbg_constr e;
+      (* FIXME: try to keep identifier for function name *)
+      let e' := constr:(subst' $x $v2 (subst' $f #() $e)) in
+      Control.time (Some "simpl took: ") (fun () => Std.eval_simpl simpl_flags None e')
+      (* XXX: simplifying [subst']; should try implementing this directly in
+         Ltac2, as it takes up nearly all the time. *)
+  | App (?e1) (Val ?v)  =>
+      dbg (of_string "reached App e v");
+      let e1 := expr_step '$e1 in
+      '(App $e1 (Val $v))
+  | App ?e1 ?e2 =>
+      dbg (of_string "reached App e e");
+      let e2new := expr_step '$e2 in
+      dbg_constr e2new;
+      '(App $e1 $e2new)
+  end
+.
+
+Ltac2 rec expr_steps e : constr :=
+  Control.plus
+    (fun () => expr_steps (expr_step e))
+    (fun ex => print (of_string "no more steps due to: "); print (of_exn ex); e)
+.
+
+Context `{!heapGS Σ}.
+Lemma wp_LockClerk__Lock (ck : loc) key R :
+  {{{
+       True
+  }}}
+    LockClerk__Lock #ck #(str key)
+  {{{
+       RET #(); R
+  }}}
+.
+Proof.
+  iIntros (?) "? HΦ".
+  wp_rec.
+  (* time wp_pures. (* ~50-70ms *) *)
+  Proof Mode "Ltac2".
+  Ltac2 Set dbg := (fun _ => ()).
+  Ltac2 Set dbg_constr := (fun _ => ()).
+  Time match! goal with
+  | [ |- envs_entails ?Δ (wp ?s ?et ?e ?Φ)] =>
+      let e' := (expr_steps e) in
+      enough (envs_entails $Δ (wp $s $et $e' $Φ)) by admit
+  end.
+  (* 5ms for simpl (which can likely be reduced), 6ms total. *)
+  Proof Mode "Classic".
+  wp_alloc ck_ptr as "?".
+  wp_alloc k as "?".
+  wp_pures.
+Admitted.
